# Circle Theorems

**1** **Angle subtended at the arc is twice the angle subtended at the circumference**

![Theorem 1](https://www.mathematics-monster.com/images5/circle_theorem_angle_at_center_twice_angle_at_circumference.jpg)

**2** **The angle subtended inside a semi-circle is a right angle**

![Theorem 2](https://www.mathematics-monster.com/images5/circle_theorem_angle_in_semicircle_is_90_degrees.jpg)

**3** **Opposite angles in a cyclic quadrilateral are supplementary**

![Theorem 3](https://www.mathematics-monster.com/images5/circle_theorem_opposite_angles_in_a_cyclic_quadrilateral_add_up_to_180_degrees.jpg)

**4** **Tangents drawn from outside points create 2 congruent right-angled triangles**

![Theorem 4](https://www.mathematics-monster.com/images5/circle_theorem_tangents_from_same_point_are_equal.jpg)

**5)** **Angle between a chord and tangent equal to angle subtended at circumference in opposite segment**

![Theorem 5](https://www.mathematics-monster.com/images5/circle_theorem_angle_in_alternate_segment_is_equal.jpg)

# Graph transformations
```
y = f(x) + a
```

Translate graph by vector **(<sup>0</sup><sub>a</sub>)**

![Vertical translation](https://img.sparknotes.com/figures/5/585483eda45473ee0e63740d71a1ae7a/vertical_shift.gif)

```
y = f(x + b)
```

Translate graph by vector  **(<sup>-b</sup><sub>0</sub>)**

![Horizantal translation](https://img.sparknotes.com/figures/5/585483eda45473ee0e63740d71a1ae7a/horizontal_shift.gif)

```
y = cf(x)
```

Stretch graph by **c** in the y-axis (Amplitude)

![Amplitude](https://s3-us-west-2.amazonaws.com/courses-images/wp-content/uploads/sites/896/2016/10/18203611/CNX_Precalc_Figure_01_05_0242.jpg)

```
y = f(kx)
```

Stretch graph by **(<sup>1</sup>/<sub>k</sub>)** in x-axis (Frequency)

![Frequency](https://s3-us-west-2.amazonaws.com/courses-images/wp-content/uploads/sites/896/2016/10/18203621/CNX_Precalc_Figure_01_05_028.jpg)

# Proving the Quadratic Formula

Start with the general equation of ax<sup>2</sup> + bx + c = 0

**ax<sup>2</sup> + bx + c = 0**

**x<sup>2</sup> + <sup>b</sup>⁄<sub>a</sub>x + <sup>c</sup>⁄<sub>a</sub> = 0**

**x<sup>2</sup> + <sup>b</sup>⁄<sub>a</sub>x = -<sup>c</sup>⁄<sub>a</sub>**

**(x + <sup>b</sup>⁄<sub>2a</sub>)<sup>2</sup> - (<sup>b</sup>⁄<sub>2a</sub>)<sup>2</sup> = -<sup>c</sup>⁄<sub>a</sub>**

# Quadratics

Quadratic equations can be solved in 3 ways.

## Method 1) Factorisation
```

```

## Method 2) Completing the Square
```

```

## Method 3) Using the formula
```

```

# Simultaneous Equations

Solved in 2 ways.

## Method 1) Elimination

4x + 3y = 18

 x - 3y = 7

Adding both equations together to eliminate y we get:

5x     = 25

∴ x = 5

So x is subsituted in any other equation to find y

(5) - 3y = 7

(5) - 7 = 3y

<sup>-2</sup> / <sub>3</sub> = y

∴ y = -2/3



## Method 2) Subsitution

2x + 3y =  9.95

 x + 4y = 10.35
 
So we rearrange one of them to subsitute into the other:

2x + 3y =  9.95

 x = 10.35 - 4y

So now subsitute second equation into first one:

≡ 2(10.35 - 4y) + 3y = 9.95

20.70 - 8y + 3y = 9.95

20.70 - 5y = 9.95

20.70 = 9.95 + 5y

20.70 - 9.95 = 5y

10.75 = 5y

∴ y = 2.15

Now we subsitute this into any equation to find x

x + 4(2.15) = 10.35

x = 10.35 - 4(2.15)

∴ x = 1.75

# Surds

Has (this many) rules/laws.
